code/experimental/ed25519/Hacl.Impl.Ed25519.RecoverX.fst
@@ -1,26 +1,138 @@
 module Hacl.Impl.Ed25519.RecoverX
 
 open FStar.Buffer
+open FStar.UInt64
 open Hacl.Spec.BignumQ.Eval
 
-let qelemB = b:buffer Hacl.UInt64.t{length b = 5}
+let elemB = b:buffer Hacl.UInt64.t{length b = 5}
+
+private
+val recover_x_step_1:
+  x2:elemB ->
+  y:elemB ->
+  Stack unit
+    (requires (fun h -> live h x2 /\ live h y))
+    (ensures (fun h0 _ h1 -> live h1 x2 /\ live h0 y /\ modifies_1 x2 h0 h1))
+let recover_x_step_1 x2 y =
+  push_frame();
+  let zero = (Hacl.Cast.uint64_to_sint64 0uL) in
+  let one' = (Hacl.Cast.uint64_to_sint64 1uL) in
+  let tmp = create (Hacl.Cast.uint64_to_sint64 0uL) 25ul in
+  let one = Buffer.sub tmp 0ul 5ul in
+  let y2  = Buffer.sub tmp 5ul 5ul in
+  let dyyi = Buffer.sub tmp 10ul 5ul in
+  let dyy = Buffer.sub tmp 15ul 5ul in
+  Hacl.Lib.Create64.make_h64_5 one one' zero zero zero zero;
+  Hacl.Bignum25519.fsquare y2 y;
+  Hacl.Bignum25519.times_d dyy y2;
+  Hacl.Bignum25519.fsum dyy one;
+  Hacl.Bignum25519.inverse dyyi dyy;
+  Hacl.Bignum25519.fdifference one y2;
+  Hacl.Bignum25519.fmul x2 one dyyi;
+  Hacl.Bignum25519.reduce x2;  
+  pop_frame()
+
+
+(* val compare: *)
+(*   x:elemB -> *)
+(*   y:elemB -> *)
+(*   Stack bool *)
+(*     (requires (fun h -> live h x /\ live h y)) *)
+(*     (ensures (fun h0 b h1 -> h0 == h1 /\ live h0 x /\ live h0 y /\ *)
+(*       b <==> (as_seq h0 x == as_seq h0 y))) *)
+(* let compare x y = *)
+(*   let x0 = x.(0ul) in *)
+(*   let x1 = x.(1ul) in *)
+(*   let x2 = x.(2ul) in *)
+(*   let x3 = x.(3ul) in *)
+(*   let x4 = x.(4ul) in *)
+(*   let y0 = y.(0ul) in *)
+(*   let y1 = y.(1ul) in *)
+(*   let y2 = y.(2ul) in *)
+(*   let y3 = y.(3ul) in *)
+(*   let y4 = y.(4ul) in *)
+(*   FStar.UInt64.(x0 =^ y0 && x1 =^ y1 && x2 =^ y2 && x3 =^ y3 && x4 =^ y4) *)
+
+private
+val is_0:
+  x:elemB ->
+  Stack bool
+    (requires (fun h -> live h x /\ Hacl.Bignum25519.red_51 (as_seq h x)))
+    (ensures (fun h0 b h1 -> h0 == h1 /\ live h0 x /\
+      b <==> (Hacl.Spec.Bignum.Bigint.seval (as_seq h0 x) == 0)))
+let is_0 x =
+  let x0 = x.(0ul) in
+  let x1 = x.(1ul) in
+  let x2 = x.(2ul) in
+  let x3 = x.(3ul) in
+  let x4 = x.(4ul) in
+  FStar.UInt64.(x0 =^ 0uL && x1 =^ 0uL && x2 =^ 0uL && x3 =^ 0uL && x4 =^ 0uL)
+
+private
+val mul_modp_sqrt_m1:
+  x:elemB ->
+  Stack unit
+    (requires (fun h -> live h x /\ Hacl.Bignum25519.red_51 (as_seq h x) ))
+    (ensures (fun h0 _ h1 -> live h1 x /\ live h0 x /\ modifies_1 x h0 h1
+      /\ Hacl.Bignum25519.red_51 (as_seq h0 x) /\ Hacl.Bignum25519.red_51 (as_seq h1 x) /\
+      Hacl.Spec.Bignum.Bigint.seval (as_seq h1 x)
+      == Spec.Curve25519.(Hacl.Spec.Bignum.Bigint.seval (as_seq h0 x) `fmul` (Spec.Ed25519.modp_sqrt_m1))
+    ))
+let mul_modp_sqrt_m1 x =
+  push_frame();
+  let sqrt_m1 = create 0uL 5ul in
+  Hacl.Lib.Create64.make_h64_5 sqrt_m1 0x00061b274a0ea0b0uL 0x0000d5a5fc8f189duL 0x0007ef5e9cbd0c60uL 0x00078595a6804c9euL 0x0002b8324804fc1duL;
+  Hacl.Bignum25519.fmul x x sqrt_m1;
+  Hacl.Bignum25519.reduce x;
+  pop_frame()
+
 
 val recover_x:
-  x:qelemB ->
-  y:qelemB{disjoint x y} ->
+  x:elemB ->
+  y:elemB{disjoint x y} ->
   sign:Hacl.UInt64.t ->
-  Stack FStar.UInt32.t
+  Stack bool
     (requires (fun h -> live h x /\ live h y))
     (ensures (fun h0 _ h1 -> live h1 x /\ live h0 y /\ modifies_1 x h0 h1))
 let recover_x x y sign =
   push_frame();
-  let m = create 0uL 5ul in
-  let m = Hacl.Impl.BignumQ.Mul.make_m m in
-  Hacl.Impl.BignumQ.Mul.subm_conditional x y m;
+  let tmp = create 0uL 20ul in
+  let x2  = Buffer.sub tmp 0ul 5ul in
+  let x3  = Buffer.sub tmp 5ul 5ul in
+  let t0  = Buffer.sub tmp 10ul 5ul in
+  let t1  = Buffer.sub tmp 15ul 5ul in
+  Hacl.Impl.BignumQ.Mul.subm_conditional x y;
   let x4 = x.(4ul) in
   let res =
-  if FStar.UInt64 (x4 >= 0x10000000000uL) then 1uL
+  if x4 >=^ 0x10000000000uL then false
   else (
-    // Compute ((y `fmul` y) `fsub` 1) `fmul` (modp_inv ((d `fmul` y `fmul` y) `fadd` one))
-    
-  )
+    recover_x_step_1 x2 y;
+    Hacl.Impl.Ed25519.Pow2_252m2.pow2_252m2 x3 x2;
+    Hacl.Bignum25519.fsquare t0 x3;
+    blit x2 0ul t1 0ul 5ul;
+    Hacl.Bignum25519.fdifference t1 t0;
+    Hacl.Bignum25519.reduce t1;
+    let t1_is_0 = is_0 t1 in
+    if t1_is_0 then ()
+    else (
+      mul_modp_sqrt_m1 x3
+    );
+    Hacl.Bignum25519.fsquare t0 x3;
+    blit x2 0ul t1 0ul 5ul;
+    Hacl.Bignum25519.fdifference t1 t0;
+    Hacl.Bignum25519.reduce t1;
+    let t1_is_0 = is_0 t1 in
+    if t1_is_0 then (
+      let x0 = x3.(0ul) &^ 1uL in
+      if not(x0 =^ sign) then (
+        Hacl.Lib.Create64.make_h64_5 t0 0uL 0uL 0uL 0uL 0uL;
+        Hacl.Bignum25519.fdifference x3 t0;
+        Hacl.Bignum25519.reduce x3
+      ) else ();
+      blit x3 0ul x 0ul 5ul;
+      true
+    )
+    else false
+  ) in
+  pop_frame();
+  res
